listimport/importfile1.v
@@ -1,5 +1,0 @@
-Require Import List.
-
-Goal forall P, P -> P.
-  easy.
-Qed.
