listimport/importfile2.v
@@ -1,7 +1,0 @@
-From ASUB Require Import importfile1.
-
-(* ssreflect rewrite due to List import is transitive *)
-Goal forall P Q, P <-> Q -> P -> Q.
-Proof.
-  intros P Q H. rewrite H. easy.
-Qed.
