listimport/localimport1.v
@@ -1,9 +1,0 @@
-Require List. 
-
-Module proofs.
-
-  Goal forall P Q, P <-> Q -> P -> Q.
-    intros P Q H. rewrite H. easy.
-  Qed.
-
-End proofs.
