listimport/myrewrite1.v
@@ -1,2 +1,0 @@
-
-Ltac myrewrite H := rewrite H.
