src/GenUps.v
@@ -6,11 +6,11 @@ Import ListNotations.
 From MetaCoq.Template Require Import All.
 From ASUB Require Import Language Utils Flags.
 
-(** * Generate all the liftings (\fatarrow^y_x) for all pairs of sorts in the current component.
+(** * Generate all the liftings (\fatarrow^y_x) for all pairs of sorts in the given substitution vector.
  ** So that we can later build the lifting functions
  ** e.g. "X_ty_ty", "X_ty_vl" etc. *)
-Definition getUps (component: list tId) (remove: list (tId * tId)) (sc: scope_type) : list (tId * tId) * list (Binder * tId) :=
-  let cart := cartesian_product component component in
+Definition getUps (substSorts: list tId) (remove: list (tId * tId)) (sc: scope_type) : list (tId * tId) * list (Binder * tId) :=
+  let cart := cartesian_product substSorts substSorts in
   let cart := list_diff_prod cart remove in
   let singles := map (fun '(x, y) => (Single x, y)) cart in
   let blists := map (fun '(x, y) => (BinderList "p" x, y)) cart in
@@ -19,3 +19,28 @@ Definition getUps (component: list tId) (remove: list (tId * tId)) (sc: scope_ty
   | Wellscoped => (cart, List.app singles blists)
   end.
 
+From ASUB Require Import GenM.
+Import GenM.Notations GenM.
+
+Definition getUps' (_: unit) : GenM.t (list (list (Binder * tId))) :=
+  sc <- get_scope_type;;
+  components <- asks (fun x => x.(R_sig).(sigComponents));;
+  substSortsByComponent <- a_map (fun c => substOf (NEList.hd c)) components;;
+  let '(_, upsByComponent) :=
+    List.fold_left (fun '(doneUps, ups) substSorts =>
+                      let '(newDoneUps, newUps) := getUps substSorts doneUps sc in
+                      (List.app doneUps newDoneUps, List.app ups [newUps]))
+                   substSortsByComponent
+                   ([], []) in
+  pure upsByComponent.
+
+Definition getUpsPure (_: unit) : GenM.t (list (list (tId * tId))) :=
+  components <- asks (fun x => x.(R_sig).(sigComponents));;
+  substSortsByComponent <- a_map (fun c => substOf (NEList.hd c)) components;;
+  let '(_, upsByComponent) :=
+    List.fold_left (fun '(doneUps, ups) substSorts =>
+                      let '(newDoneUps, _) := getUps substSorts doneUps Unscoped in
+                      (List.app doneUps newDoneUps, List.app ups [newDoneUps]))
+                   substSortsByComponent
+                   ([], []) in
+  pure upsByComponent.
