src/static/unscoped_axioms.v
@@ -1,4 +1,4 @@
-Require Import core core_axioms unscoped.
+From ASUB Require Import core core_axioms unscoped.
 Import UnscopedNotations.
 
 (** Eta laws. *)
